Automata

src/ASN1/ASN1.Spec.Automata.fst
@@ -3,121 +3,7 @@ module ASN1.Spec.Automata
 open LowParse.Spec.Base
 open LowParse.Spec.Combinators
 
-open LowParse.Spec.Int
-
-open FStar.Mul
-
-module U8 = FStar.UInt8
-module U32 = FStar.UInt32
-module Cast = FStar.Int.Cast
-
 open ASN1.Base
-
-let id_cast
-  (t : eqtype)
-  (p1 : t -> Type0)
-  (p2 : t -> Type0)
-  (lem : (x : t -> (Lemma (p1 x ==> p2 x))))
-  (x : t {p1 x})
-: (x' : t {p2 x'})
-= let _ = lem x in
-  (x <: (x : t {p2 x}))
-
-let parse_cast
-  (t : eqtype)
-  (p1 : t -> Type0)
-  (p2 : t -> Type0)
-  (lem : (x : t -> (Lemma (p1 x ==> p2 x))))
-  (#k : parser_kind)
-  (p : parser k (x: t {p1 x}))
-: (parser k (x : t {p2 x}))
-= parse_synth #k #(x : t{p1 x}) #(x : t{p2 x}) p (id_cast t p1 p2 lem)
-
-let parse_cast_eq
-  (t : eqtype)
-  (p1 : t -> Type0)
-  (p2 : t -> Type0)
-  (lem : (x : t -> (Lemma (p1 x ==> p2 x))))
-  (#k : parser_kind)
-  (p : parser k (x : t {p1 x}))
-  (b : bytes)
-: Lemma (ensures (parse (parse_cast t p1 p2 lem p) b = (match (parse p b) with
-                                                       | None -> None
-                                                       | Some (x, l) -> Some (id_cast t p1 p2 lem x, l))))
-= parse_synth_eq #k #(x : t{p1 x}) #(x : t{p2 x}) p (id_cast t p1 p2 lem) b
-
-let parse_cast_inverse
-  (t : eqtype)
-  (p1 : t -> Type0)
-  (p2 : t -> Type0)
-  (lem : (x : t -> (Lemma (p1 x ==> p2 x))))
-  (#k : parser_kind)
-  (p : parser k (x : t {p1 x}))
-  (b : bytes)
-  (x : t {p2 x})
-  (l : consumed_length b)
-: Pure (x : t {p1 x})
-  (requires (parse (parse_cast t p1 p2 lem p) b = Some (x, l)))
-  (ensures (fun y -> y = x))
-= let _ = parse_cast_eq t p1 p2 lem p b in
-  match (parse p b) with
-  | Some (x, l) -> x
-
-let cases_injective2_precond
-  (#t1 #t2:Type)
-  (#t': Type)
-  (gt : t1 -> t' -> Type0)
-  (p': ((x : t1) -> t2 -> Tot (bare_parser (y : t' {gt x y}))))
-  (x1 x2: t1)
-  (y1 y2: t2)
-  (b1 b2: bytes)
-: GTot Type0
-= Some? (parse (p' x1 y1) b1) /\
-  Some? (parse (p' x2 y2) b2) /\ (
-    let (Some (v1, _)) = parse (p' x1 y1) b1 in
-    let (Some (v2, _)) = parse (p' x2 y2) b2 in
-    v1 == v2
-  )
-
-let cases_injective2
-  (#t1 #t2:Type)
-  (#t': Type)
-  (gt : t1 -> t' -> Type0)
-  (p': ((x : t1) -> t2 -> Tot (bare_parser (y : t' {gt x y}))))
-: GTot Type0
-= forall (x1 x2: t1) (y1 y2 : t2) (b1 b2: bytes) . {:pattern (parse (p' x1 y1) b1); (parse (p' x2 y2) b2)}
-  cases_injective2_precond gt p' x1 x2 y1 y2 b1 b2 ==>
-  x1 == x2 /\ y1 == y2
-
-let cases_injective2_intro
-  (#t1 #t2:Type)
-  (#t': Type)
-  (gt : t1 -> t' -> Type0)
-  (p': ((x : t1) -> t2 -> Tot (bare_parser (y : t' {gt x y}))))
-  (lem: (
-    (x1: t1) -> 
-    (x2: t1) ->
-    (y1 : t2) ->
-    (y2 : t2) ->
-    (b1: bytes) ->
-    (b2: bytes) ->
-    Lemma
-    (requires (cases_injective2_precond gt p' x1 x2 y1 y2 b1 b2))
-    (ensures (x1 == x2 /\ y1 == y2))
-  ))
-: Lemma
-  (cases_injective2 gt p')
-= Classical.forall_intro (fun x1 -> Classical.forall_intro_4 (fun x2 y1 y2 b1 -> Classical.forall_intro (Classical.move_requires (lem x1 x2 y1 y2 b1))))
-
-let cases_injective2_weaken
-  (#t1 #t2:Type)
-  (#t': Type)
-  (gt : t1 -> t' -> Type0)
-  (p': ((x : t1) -> t2 -> Tot (bare_parser (y : t' {gt x y}))))
-: Lemma
-  (requires cases_injective2 gt p')
-  (ensures (forall (x : t1). and_then_cases_injective (p' x)))
-= _
 
 noeq
 type automata_control_param = {
@@ -129,6 +15,8 @@ type automata_control_param = {
   next_state : (s : control_t) ->
                (ch : ch_t {fail_check s ch = false /\ termination_check s ch = false}) -> control_t;
 }
+
+(*
 
 type extend_control_t (t : Type) =
 | CFail 
@@ -164,29 +52,7 @@ let rec automata_cp_big_step_list
     | CCont s' -> automata_cp_big_step_list cp s' tl
     | other -> other
 
-type dec (t : Type) = nat -> option t
-
-(*
-let dec_count (t : Type) (c : dec t) : dec t =
-  fun n -> if n = 0 then
-          None
-        else 
-          c (n - 1)
 *)
-
-let rec dec_fix'
-  (s : Type)
-  (t : Type)
-  (f : s -> (k : nat) -> (s -> ((m : nat {m <= k}) -> option t)) -> option t)
-  (x : s)
-  (n : nat)
-: Tot (option t)
-  (decreases n)
-= if n = 0 then
-    None
-  else 
-    f x (n - 1) (fun y (m : nat {m <= n - 1}) -> dec_fix' s t f y m) 
-
 
 noeq
 type automata_data_param (cp : automata_control_param) = {
@@ -211,6 +77,7 @@ type automata_data_param (cp : automata_control_param) = {
                    (post_t (cp.next_state state ch) (update_next state data ch) ret ==> post_t state data ret)
 }
 
+(*
 type extend_control_data_t
   (cp : automata_control_param)
   (dp : automata_data_param cp)
@@ -232,15 +99,26 @@ let automata_cp_dp_small_step
       DTerm (dp.update_term s data ch)
     else 
       DCont (cp.next_state s ch) (dp.update_next s data ch)
+*)     
 
 noeq
 type automata_bare_parser_param (cp : automata_control_param) = {
   ch_t_bare_parser : bare_parser cp.ch_t;
-  ch_t_bare_parser_valid : 
-    (forall (b : bytes). match (parse ch_t_bare_parser b) with
+  ch_t_bare_parser_valid : ((b : bytes) ->
+    Lemma (match (parse ch_t_bare_parser b) with
                     | Some (_, n) -> n > 0
-                    | None -> True);
+                    | None -> True))
 }
+
+let id_cast
+  (t : eqtype)
+  (p1 : t -> Type0)
+  (p2 : t -> Type0)
+  (lem : (x : t -> (Lemma (p1 x ==> p2 x))))
+  (x : t {p1 x})
+: (x' : t {p2 x'})
+= let _ = lem x in
+  (x <: (x : t {p2 x}))
 
 let rec automata_bare_parser'
   (cp : automata_control_param)
@@ -249,7 +127,7 @@ let rec automata_bare_parser'
   (s : cp.control_t)
   (data : dp.partial_t {dp.pre_t s data})
   (b : bytes)
-: Tot (option (tuple2 (ret : dp.ret_t {dp.post_t s data ret}) (consumed_length b)))
+: Tot (option ((ret : dp.ret_t {dp.post_t s data ret}) * (consumed_length b)))
   (decreases (Seq.length b))
 = match (parse bp.ch_t_bare_parser b) with
   | None -> None
@@ -263,7 +141,7 @@ let rec automata_bare_parser'
         (
         let s' = cp.next_state s ch in
         let data' = dp.update_next s data ch in
-        let _ = bp.ch_t_bare_parser_valid in
+        let _ = bp.ch_t_bare_parser_valid b in
         let (b' : bytes{Seq.length b' < Seq.length b}) = Seq.slice b l (Seq.length b) in
         match (automata_bare_parser' cp dp bp s' data' b') with
         | None -> None
@@ -271,451 +149,326 @@ let rec automata_bare_parser'
           Some (id_cast dp.ret_t (dp.post_t s' data') (dp.post_t s data) (dp.lemma_cast_ret s data ch) ret, l + l')
         )
 
-let automata_bare_parser
+type automata_default_parser_kind : parser_kind = {
+  parser_kind_metadata = None;
+  parser_kind_low = 0;
+  parser_kind_high = None;
+  parser_kind_subkind = Some ParserStrong;
+}
+
+noeq
+type automata_parser_param (cp : automata_control_param) (dp : automata_data_param cp) (bp : automata_bare_parser_param cp) = {
+  ch_t_parser_valid : unit -> Lemma (parser_kind_prop automata_default_parser_kind bp.ch_t_bare_parser);
+
+  lemma_update_term_inj2 : ((state : cp.control_t) -> 
+    (data1 : dp.partial_t {dp.pre_t state data1}) ->
+    (data2 : dp.partial_t {dp.pre_t state data2}) ->
+    (ch1 : cp.ch_t {cp.fail_check state ch1 = false /\ cp.termination_check state ch1 = true}) ->
+    (ch2 : cp.ch_t {cp.fail_check state ch2 = false /\ cp.termination_check state ch2 = true}) ->
+    Lemma (requires (dp.update_term state data1 ch1 = dp.update_term state data2 ch2))
+          (ensures (data1 = data2 /\ ch1 = ch2)));
+
+  lemma_update_term_next_non_intersect : ((state : cp.control_t) ->
+    (data1 : dp.partial_t {dp.pre_t state data1}) ->
+    (data2 : dp.partial_t {dp.pre_t state data2}) ->
+    (ch1 : cp.ch_t {cp.fail_check state ch1 = false /\ cp.termination_check state ch1 = true}) ->
+    (ch2 : cp.ch_t {cp.fail_check state ch2 = false /\ cp.termination_check state ch2 = false}) ->
+    (ret1 : dp.ret_t {dp.post_t state data1 ret1}) ->
+    (ret2 : dp.ret_t {dp.post_t (cp.next_state state ch2) (dp.update_next state data2 ch2) ret2}) ->
+    Lemma (requires (ret1 = dp.update_term state data1 ch1 /\ ret1 = ret2))
+          (ensures False));
+
+  lemma_update_next_non_intersect : ((state : cp.control_t) ->
+    (data1 : dp.partial_t {dp.pre_t state data1}) ->
+    (data2 : dp.partial_t {dp.pre_t state data2}) ->
+    (ch1 : cp.ch_t {cp.fail_check state ch1 = false /\ cp.termination_check state ch1 = false}) ->
+    (ch2 : cp.ch_t {cp.fail_check state ch2 = false /\ cp.termination_check state ch2 = false}) ->
+    (ret1 : dp.ret_t {dp.post_t (cp.next_state state ch1) (dp.update_next state data1 ch1) ret1}) ->
+    (ret2 : dp.ret_t {dp.post_t (cp.next_state state ch2) (dp.update_next state data2 ch2) ret2}) ->
+    Lemma (requires (cp.next_state state ch1 <> cp.next_state state ch2 /\ ret1 = ret2))
+          (ensures False));
+
+  lemma_update_next_inj2 : ((state : cp.control_t) -> 
+    (data1 : dp.partial_t {dp.pre_t state data1}) ->
+    (data2 : dp.partial_t {dp.pre_t state data2}) ->
+    (ch1 : cp.ch_t {cp.fail_check state ch1 = false /\ cp.termination_check state ch1 = false}) ->
+    (ch2 : cp.ch_t {cp.fail_check state ch2 = false /\ cp.termination_check state ch2 = false}) ->
+    Lemma (requires cp.next_state state ch1 = cp.next_state state ch2 /\ dp.update_next state data1 ch1 = dp.update_next state data2 ch2)
+          (ensures data1 = data2 /\ ch1 = ch2))
+}
+
+let and_then_cases_injective_dep_precond
+  (#t:Type)
+  (#t': Type)
+  (gt : t -> t' -> Type0)
+  (p': ((x : t) -> Tot (bare_parser (y : t' {gt x y}))))
+  (x1 x2: t)
+  (b1 b2: bytes)
+: GTot Type0
+= Some? (parse (p' x1) b1) /\
+  Some? (parse (p' x2) b2) /\ (
+    let (Some (v1, _)) = parse (p' x1) b1 in
+    let (Some (v2, _)) = parse (p' x2) b2 in
+    v1 == v2
+  )
+
+let and_then_cases_injective_dep
+  (#t : Type)
+  (#t' : Type)
+  (gt : t -> t' -> Type0)
+  (p': ((m : t) -> Tot (bare_parser (x : t' {gt m x}))))
+: GTot Type0
+= forall (x1 x2: t) (b1 b2: bytes) . {:pattern (parse (p' x1) b1); (parse (p' x2) b2)}
+  and_then_cases_injective_dep_precond gt p' x1 x2 b1 b2 ==>
+  x1 == x2
+
+let and_then_cases_injective_dep_intro
+  (#t : Type)
+  (#t': Type)
+  (gt : t -> t' -> Type0)
+  (p': ((x : t) -> Tot (bare_parser (y : t' {gt x y}))))
+  (lem: (
+    (x1: t) -> 
+    (x2: t) ->
+    (b1: bytes) ->
+    (b2: bytes) ->
+    Lemma
+    (requires (and_then_cases_injective_dep_precond gt p' x1 x2 b1 b2))
+    (ensures (x1 == x2))
+  ))
+: Lemma
+  (and_then_cases_injective_dep gt p')
+= Classical.forall_intro_4 (fun x1 x2 b1 b2 -> (Classical.move_requires (lem x1 x2 b1) b2))
+
+let rec automata_bare_parser'_pf1_aux
   (cp : automata_control_param)
   (dp : automata_data_param cp)
   (bp : automata_bare_parser_param cp)
+  (pp : automata_parser_param cp dp bp)
   (s : cp.control_t)
-  (data : dp.partial_t {dp.pre_t s data})
-: (bare_parser (ret : dp.ret_t {dp.post_t s data ret}))
-= automata_bare_parser' cp dp bp s data
-
-(*
-
-noeq
-type automata_parser_param (cp : automata_control_param) (dp : automata_data_param cp) = {
-  ch_t_parser_kind : parser_kind;
-  ch_t_parser : parser ch_t_parser_kind cp.ch_t;
-  ch_t_parser_valid : 
-    (forall (b : bytes). match (parse ch_t_parser b) with
-                    | Some (_, n) -> n > 0
-                    | None -> True);
-                          
-}
-*) 
-
-(*
-  ch_t_parser_kind : parser_kind;
-  ch_t_parser : parser ch_t_parser_kind cp.ch_t;
-
-
-*)
-
-(*
-
-// Control plane
-
-// assume val control_t : eqtype
-
-type control_t =
-| Init | S3' | S3 | S2' | S2 | S1
-
-let ord (s : control_t) : nat =
-  match s with
-  | S1 -> 0
-  | S2 | S2' -> 1
-  | S3 | S3' -> 2
-  | Init -> 3
-
-// assume val ch_t : eqtype
-
-let ch_t = U8.t
-
-//  assume val ch_t_parser_kind : parser_kind
-
-let ch_t_parser_kind = parse_u8_kind
-
-// assume val ch_t_parser : parser ch_t_parser_kind ch_t
-
-let ch_t_parser : parser ch_t_parser_kind ch_t = parse_u8
-
-// assume val fail_check : control_t -> ch_t -> bool
-
-let out_range_common (ch : ch_t) =
-  U8.v ch < 128 || 128 + 64 <= U8.v ch
-
-let out_range_s2' (ch : ch_t) =
-  U8.v ch < 128 + 32 || 128 + 64 <= U8.v ch
-
-let out_range_s3' (ch : ch_t) =
-  U8.v ch < 128 + 16 || 128 + 64 <= U8.v ch
-
-let out_range_init (ch : ch_t) =
-  (128 <= U8.v ch && U8.v ch <= 128 + 64) || 248 <= U8.v ch
-
-let fail_check (s : control_t) : ch_t -> bool =
-  match s with
-  | S1 | S2 | S3 -> out_range_common
-  | S2' -> out_range_s2'
-  | S3' -> out_range_s3'
-  | Init -> out_range_init
-
-// assume val terminate_check : (state : control_t) -> (ch : ch_t {fail_check state ch = false}) -> bool
-
-let terminate_check (s : control_t) =
-  match s with
-  | S1 -> fun _ -> true
-  | S2 | S3 | S2' | S3' -> fun _ -> false
-  | Init -> (fun (ch : ch_t {fail_check s ch = false}) -> U8.v ch < 128)
-
-// assume val next_state : (state : control_t) -> (ch : ch_t {fail_check state ch = false /\ terminate_check state ch = false}) -> (state' : control_t {state' << state})
-
-let next_state (s : control_t) (ch : ch_t {fail_check s ch = false /\ terminate_check s ch = false}) : (s' : control_t {ord s' << ord s}) =
-  match s with
-  | S2 | S2' -> S1
-  | S3 | S3' -> S2
-  | Init -> if (U8.v ch < 128 + 64 + 32) then
-             S1
-           else if (U8.v ch = 128 + 64 + 32) then
-             S2'
-           else if (U8.v ch < 128 + 64 + 32 + 16) then
-             S2
-           else if (U8.v ch = 128 + 64 + 32 + 16) then
-             S3'
-           else
-             S3
-
-// Data plane
-
-// assume val ret_t : eqtype
-
-let ret_t = U32.t
-
-// assume val partial_t : eqtype
-
-let partial_t = U32.t
-  
-// assume val pre_t : control_t -> partial_t -> Type0
-
-let pre_t (s : control_t) : partial_t -> Type0 =
-  match s with
-  | S1 -> (fun data -> 0 < U32.v data /\ U32.v data < pow2 26)
-  | S2 -> (fun data -> 0 < U32.v data /\ U32.v data < pow2 20)
-  | S3 -> (fun data -> 0 < U32.v data /\ U32.v data < pow2 14)
-  | S2' | S3' | Init -> (fun data -> U32.v data = 0)
-
-// assume val post_t : (s : control_t) -> (data : partial_t {pre_t s data}) -> ret_t -> Type0
-
-let post_t (s : control_t) (data : partial_t {pre_t s data}) : ret_t -> Type0 =
-  match s with
-  | S1 -> (fun data' -> U32.v data * (pow2 6) <= U32.v data' /\ U32.v data' < (U32.v data + 1) * (pow2 6))
-  | S2 -> (fun data' -> U32.v data * (pow2 12) <= U32.v data' /\ U32.v data' < (U32.v data + 1) * (pow2 12))
-  | S3 -> (fun data' -> U32.v data * (pow2 18) <= U32.v data' /\ U32.v data' < (U32.v data + 1) * (pow2 18))
-  | S2' -> (fun data' -> pow2 11 <= U32.v data' /\ U32.v data' < pow2 12)
-  | S3' -> (fun data' -> pow2 16 <= U32.v data' /\ U32.v data' < pow2 18)
-  | Init -> (fun data' -> U32.v data' < pow2 21)
-
-// assume val ret_t_parser_kind : control_t -> parser_kind
-
-let ret_t_parser_kind (s : control_t) : parser_kind = asn1_strong_parser_kind
-
-//assume val update_term : (state : control_t) -> (data : partial_t {pre_t state data}) -> 
-//  (ch : ch_t {fail_check state ch = false /\ terminate_check state ch = true}) -> 
-//  (ret : ret_t {post_t state data ret}) 
-
-let update_term (state : control_t) : (data : partial_t {pre_t state data}) -> 
-  (ch : ch_t {fail_check state ch = false /\ terminate_check state ch = true}) -> 
-  (ret : ret_t {post_t state data ret}) =
-  match state with
-  | S2 | S3 | S2' | S3' -> (fun _ _ -> false_elim ())
-  | S1 -> (fun data ch -> let b = U8.sub ch 128uy in (U32.add (U32.mul data 64ul) (Cast.uint8_to_uint32 b)))
-  | Init -> (fun _ ch -> Cast.uint8_to_uint32 ch)
-
-assume val lemma_update_term_inj2 (state : control_t) 
-  (data1 : partial_t {pre_t state data1})
-  (data2 : partial_t {pre_t state data2})
-  (ch1 : ch_t {fail_check state ch1 = false /\ terminate_check state ch1 = true})
-  (ch2 : ch_t {fail_check state ch2 = false /\ terminate_check state ch2 = true})
-: Lemma (requires (update_term state data1 ch1 = update_term state data2 ch2))
-        (ensures (data1 = data2 /\ ch1 = ch2))
-
-//assume val update_next : (state : control_t) -> (data : partial_t {pre_t state data}) ->
-//  (ch : ch_t {fail_check state ch = false /\ terminate_check state ch = false}) ->
-//  (data' : partial_t {pre_t (next_state state ch) data'})
-
-let update_next (state : control_t) : (data : partial_t {pre_t state data}) ->
-  (ch : ch_t {fail_check state ch = false /\ terminate_check state ch = false}) ->
-  (data' : partial_t {pre_t (next_state state ch) data'}) =
-  match state with
-  | S1 -> (fun _ _ -> false_elim ())
-  | S2 -> (fun data ch ->
-           let _ = Math.Lemmas.pow2_plus 20 6 in
-           let b = U8.sub ch 128uy in (U32.add (U32.mul data 64ul) (Cast.uint8_to_uint32 b)))
-  | S3 -> (fun data ch ->
-           let _ = Math.Lemmas.pow2_plus 14 6 in
-           let b = U8.sub ch 128uy in (U32.add (U32.mul data 64ul) (Cast.uint8_to_uint32 b)))
-  | S2' -> (fun _ ch -> 
-            let b = U8.sub ch 128uy in 
-            assert (32 <= U8.v b /\ U8.v b < 64);
-            let _ = Math.Lemmas.pow2_lt_compat 26 6 in
-            Cast.uint8_to_uint32 b)
-  | S3' -> (fun _ ch -> 
-            let b = U8.sub ch 128uy in Cast.uint8_to_uint32 b)
-  | Init -> (fun _ ch -> 
-           if (U8.v ch < 128 + 64 + 32) then
-             let _ = Math.Lemmas.pow2_lt_compat 26 5 in
-             Cast.uint8_to_uint32 (U8.sub ch 192uy)
-           else if (U8.v ch = 128 + 64 + 32) then
-             0ul
-           else if (U8.v ch < 128 + 64 + 32 + 16) then
-             Cast.uint8_to_uint32 (U8.sub ch 224uy)
-           else if (U8.v ch = 128 + 64 + 32 + 16) then
-             0ul
-           else
-             Cast.uint8_to_uint32 (U8.sub ch 240uy))
-
-assume val lemma_update_term_next_non_intersect 
-  (state : control_t) 
-  (data1 : partial_t {pre_t state data1})
-  (ch1 : ch_t {fail_check state ch1 = false /\ terminate_check state ch1 = true})
-  (ch2 : ch_t {fail_check state ch2 = false /\ terminate_check state ch2 = false})
-  (ret1 : ret_t {post_t state data1 ret1})
-  (ret2 : ret_t {post_t (next_state state ch2) (update_next state data1 ch2) ret2})
-: Lemma (requires (ret1 = update_term state data1 ch1 /\ ret1 = ret2))
-        (ensures False)
-
-assume val lemma_update_next_non_intersect
-  (state : control_t) 
-  (data1 : partial_t {pre_t state data1})
-  (data2 : partial_t {pre_t state data2})
-  (ch1 : ch_t {fail_check state ch1 = false /\ terminate_check state ch1 = false})
-  (ch2 : ch_t {fail_check state ch2 = false /\ terminate_check state ch2 = false})
-  (ret1 : ret_t {post_t (next_state state ch1) (update_next state data1 ch1) ret1})
-  (ret2 : ret_t {post_t (next_state state ch2) (update_next state data2 ch2) ret2})
-: Lemma (requires (next_state state ch1 <> next_state state ch2 /\ ret1 = ret2))
-        (ensures False)
-
-assume val lemma_update_next_inj2
-  (state : control_t) 
-  (data1 : partial_t {pre_t state data1})
-  (data2 : partial_t {pre_t state data2})
-  (ch1 : ch_t {fail_check state ch1 = false /\ terminate_check state ch1 = false})
-  (ch2 : ch_t {fail_check state ch2 = false /\ terminate_check state ch2 = false})
-: Lemma (requires next_state state ch1 = next_state state ch2 /\ update_next state data1 ch1 = update_next state data2 ch2)
-        (ensures data1 = data2 /\ ch1 = ch2)
-
-assume val lemma_cast_ret (state : control_t) (data : partial_t {pre_t state data}) (ch : ch_t {fail_check state ch = false /\ terminate_check state ch = false}) (ret : ret_t)
-: Lemma (post_t (next_state state ch) (update_next state data ch) ret ==> post_t state data ret)
-
-assume val lemma_parser_kind1
-  (state : control_t)
-  (ch : ch_t {fail_check state ch = true})
-: Lemma (fail_parser_kind_precond (ret_t_parser_kind state))
-
-assume val lemma_parser_kind2
-  (state : control_t)
-  (ch : ch_t {fail_check state ch = false /\ terminate_check state ch = true})
-: Lemma (ret_t_parser_kind state `is_weaker_than` parse_ret_kind)
-
-assume val lemma_parser_kind3
-  (state : control_t)
-  (ch : ch_t {fail_check state ch = false /\ terminate_check state ch = false})
-: Lemma (ret_t_parser_kind state `is_weaker_than` (and_then_kind ch_t_parser_kind (ret_t_parser_kind (next_state state ch))))
-
-let reachable_1 (state state' : control_t) =
-  exists ch. next_state state ch = state'
-
-let lemma_reachable_1 (state state' : control_t) :
-  Lemma (requires (reachable_1 state state'))
-        (ensures (ord state' << ord state))
-= _
-
-let parse_automata_gt (state : control_t) : (data : partial_t {pre_t state data}) -> ret_t -> Type0 = fun data -> post_t state data 
-
-let parse_automata_type (state : control_t) = (data : partial_t {pre_t state data}) -> (ch : ch_t) -> parser (ret_t_parser_kind state) (ret : ret_t {parse_automata_gt state data ret})
-
-let parse_automata_spec (state : control_t) (p : parse_automata_type state)
-= cases_injective2 (parse_automata_gt state) p
-
-let parse_automata' 
-  (state : control_t)
-  (fp : (state' : control_t {reachable_1 state state'}) -> parse_automata_type state')
-  (data : partial_t {pre_t state data})
-  (ch : ch_t)
-: Pure (parser (ret_t_parser_kind state) (ret : ret_t {post_t state data ret}))
-  (requires (forall state'. parse_automata_spec state' (fp state')))
-  (ensures (fun _ -> True))
-= let k = ret_t_parser_kind state in
-  if fail_check state ch then
-    let _ = lemma_parser_kind1 state ch in
-    fail_parser k (ret : ret_t {post_t state data ret})
-  else 
-    (
-    if terminate_check state ch then
-      let _ = lemma_parser_kind2 state ch in
-      weaken k (parse_ret (update_term state data ch))
+  (x1 : dp.partial_t {dp.pre_t s x1})
+  (x2 : dp.partial_t {dp.pre_t s x2})
+  (b1 : bytes)
+  (b2 : bytes)
+: Lemma 
+  (requires (and_then_cases_injective_dep_precond (dp.post_t s) (automata_bare_parser' cp dp bp s) x1 x2 b1 b2))
+  (ensures (x1 == x2))
+  (decreases (Seq.length b1))
+= let p = automata_bare_parser' cp dp bp in
+  match (parse (p s x1) b1) with | Some (ret1, l1) ->
+  match (parse (p s x2) b2) with | Some (ret2, l2) ->
+  match (parse (bp.ch_t_bare_parser) b1) with | Some (ch1, l01) ->
+  match (parse (bp.ch_t_bare_parser) b2) with | Some (ch2, l02) ->
+  if cp.fail_check s ch1 then
+    _
+  else if cp.fail_check s ch2 then
+    _
+  else if cp.termination_check s ch1 then
+  (
+    if cp.termination_check s ch2 then
+      pp.lemma_update_term_inj2 s x1 x2 ch1 ch2 
     else
+      pp.lemma_update_term_next_non_intersect s x1 x2 ch1 ch2 ret1 ret2
+  )
+  else
+  (
+    if cp.termination_check s ch2 then
+      pp.lemma_update_term_next_non_intersect s x2 x1 ch2 ch1 ret2 ret1
+    else
+    (
+      let s'1 = cp.next_state s ch1 in
+      let s'2 = cp.next_state s ch2 in
+      let x'1 = dp.update_next s x1 ch1 in
+      let _ = bp.ch_t_bare_parser_valid b1 in
+      let (b'1 : bytes{Seq.length b'1 < Seq.length b1}) = Seq.slice b1 l01 (Seq.length b1) in
+      let x'2 = dp.update_next s x2 ch2 in
+      let _ = bp.ch_t_bare_parser_valid b2 in
+      let (b'2 : bytes{Seq.length b'2 < Seq.length b2}) = Seq.slice b2 l02 (Seq.length b2) in
+      if s'1 = s'2 then
       (
-        let state' = next_state state ch in
-        let data' = update_next state data ch in
-        let _ = cases_injective2_weaken (parse_automata_gt state') (fp state') in
-        let p = ch_t_parser `and_then` (fp state' data') in
-        let p' = 
-          parse_cast
-          ret_t
-          (post_t state' data')
-          (post_t state data)
-          (lemma_cast_ret state data ch)
-          p
-        in
-        let _ = lemma_parser_kind3 state ch in
-        weaken k p'
+        let _ = automata_bare_parser'_pf1_aux cp dp bp pp s'1 x'1 x'2 b'1 b'2 in
+        pp.lemma_update_next_inj2 s x1 x2 ch1 ch2
+      )
+      else
+      (
+        pp.lemma_update_next_non_intersect s x1 x2 ch1 ch2 ret1 ret2
       )
     )
+  )      
 
-let lemma_parse_automata'_inj2
-  (state : control_t)
-  (fp : (state' : control_t {reachable_1 state state'}) -> parse_automata_type state')  
-: Lemma (requires (forall state'. parse_automata_spec state' (fp state')))
-        (ensures (parse_automata_spec state (parse_automata' state fp)))
-= let p = parse_automata' state fp in
-  cases_injective2_intro (parse_automata_gt state) p (fun data1 data2 ch1 ch2 bytes1 bytes2 ->
-    match parse (p data1 ch1) bytes1 with | Some (ret1, l1) -> 
-    match parse (p data2 ch2) bytes2 with | Some (ret2, l2) ->   
-    if (fail_check state ch1) then
+let automata_bare_parser'_pf1
+  (cp : automata_control_param)
+  (dp : automata_data_param cp)
+  (bp : automata_bare_parser_param cp)
+  (pp : automata_parser_param cp dp bp)
+  (s : cp.control_t)
+: Lemma (and_then_cases_injective_dep (dp.post_t s) (automata_bare_parser' cp dp bp s))
+= let p = automata_bare_parser' cp dp bp s in
+  and_then_cases_injective_dep_intro (dp.post_t s) p (automata_bare_parser'_pf1_aux cp dp bp pp s)
+
+let rec automata_bare_parser'_pf2_aux
+  (cp : automata_control_param)
+  (dp : automata_data_param cp)
+  (bp : automata_bare_parser_param cp)
+  (pp : automata_parser_param cp dp bp)
+  (s : cp.control_t)
+  (x : dp.partial_t {dp.pre_t s x})
+  (b1 : bytes)
+  (b2 : bytes)
+: Lemma (requires no_lookahead_on_precond (automata_bare_parser' cp dp bp s x) b1 b2)
+        (ensures no_lookahead_on_postcond (automata_bare_parser' cp dp bp s x) b1 b2)
+        (decreases (Seq.length b1))
+= let p = automata_bare_parser' cp dp bp s x in
+  let _ = pp.ch_t_parser_valid () in
+  let _ = parser_kind_prop_equiv automata_default_parser_kind bp.ch_t_bare_parser in
+  match (parse p b1) with | Some (ret1, l1) ->
+  match (parse (bp.ch_t_bare_parser) b1) with | Some (ch1, l01) ->
+  let _ = 
+    Seq.lemma_split (Seq.slice b2 0 l1) l01;
+    Seq.lemma_split (Seq.slice b1 0 l1) l01
+  in
+  assert (Seq.slice b2 0 l01 == Seq.slice b1 0 l01);
+  match (parse (bp.ch_t_bare_parser) b2) with 
+  | None -> 
+    assert (no_lookahead_on bp.ch_t_bare_parser b1 b2)
+  | Some (ch2, l02) ->
+    assert (ch1 = ch2);
+    assert (injective_precond bp.ch_t_bare_parser b1 b2);
+    assert ((l01 <: nat) = (l02 <: nat));
+    if cp.fail_check s ch1 then
+      _
+    else if cp.termination_check s ch1 then
       _
     else
-      if (fail_check state ch2) then
-        _
-      else
-        (
-        if (terminate_check state ch1) then
-        (
-          if (terminate_check state ch2) then
-            let _ : squash (fail_check state ch1 = false /\ terminate_check state ch1 = true) = _ in
-            let _ : squash (fail_check state ch2 = false /\ terminate_check state ch2 = true) = _ in
-            lemma_update_term_inj2 state data1 data2 ch1 ch2
-          else
-          (
-            let _ : squash (fail_check state ch1 = false /\ terminate_check state ch1 = true) = _ in
-            let _ : squash (fail_check state ch2 = false /\ terminate_check state ch2 = false) = _ in
-            let state'2 = next_state state ch2 in
-            let data'2 = update_next state data2 ch2 in
-            let _ = cases_injective2_weaken (parse_automata_gt state'2) (fp state'2) in
-            let p = ch_t_parser `and_then` (fp state'2 data'2) in
-            let ret2' = 
-              parse_cast_inverse
-              ret_t
-              (post_t state'2 data'2)
-              (post_t state data2)
-              (lemma_cast_ret state data2 ch2)
-              p
-              bytes2
-              ret2
-              l2
-            in
-            lemma_update_term_next_non_intersect state data1 ch1 ch2 ret1 ret2'
-          )
-        )
-        else
-        (
-          if (terminate_check state ch2) then
-          (
-            let _ : squash (fail_check state ch1 = false /\ terminate_check state ch1 = false) = _ in
-            let _ : squash (fail_check state ch2 = false /\ terminate_check state ch2 = true) = _ in
-            let state'1 = next_state state ch1 in
-            let data'1 = update_next state data1 ch1 in
-            let _ = cases_injective2_weaken (parse_automata_gt state'1) (fp state'1) in
-            let p = ch_t_parser `and_then` (fp state'1 data'1) in
-            let ret1' = 
-              parse_cast_inverse
-              ret_t
-              (post_t state'1 data'1)
-              (post_t state data1)
-              (lemma_cast_ret state data1 ch1)
-              p
-              bytes1
-              ret1
-              l1
-            in
-            lemma_update_term_next_non_intersect state data2 ch2 ch1 ret2 ret1'
-          )
-          else
-          (
-            let _ : squash (fail_check state ch1 = false /\ terminate_check state ch1 = false) = _ in
-            let _ : squash (fail_check state ch2 = false /\ terminate_check state ch2 = false) = _ in
-            let state'1 = next_state state ch1 in
-            let state'2 = next_state state ch2 in
-            let data'1 = update_next state data1 ch1 in
-            let data'2 = update_next state data2 ch2 in
-            if (state'1 = state'2) then
-            (
-              let _ = cases_injective2_weaken (parse_automata_gt state'1) (fp state'1) in
-              let p1 = ch_t_parser `and_then` (fp state'1 data'1) in
-              let _ = parse_cast_eq
-                ret_t
-                (post_t state'1 data'1)
-                (post_t state data1)
-                (lemma_cast_ret state data1 ch1)
-                p1
-                bytes1
-              in
-              let _ = and_then_eq ch_t_parser (fp state'1 data'1) bytes1 in
-              match (parse ch_t_parser bytes1) with | Some (ch'1, l'1) -> let bytes'1 : bytes = Seq.slice bytes1 l'1 (Seq.length bytes1) in
-              let _ = cases_injective2_weaken (parse_automata_gt state'2) (fp state'2) in
-              let p2 = ch_t_parser `and_then` (fp state'2 data'2) in
-              let _ = parse_cast_eq
-                ret_t
-                (post_t state'2 data'2)
-                (post_t state data2)
-                (lemma_cast_ret state data2 ch2)
-                p2
-                bytes2
-              in
-              let _ = and_then_eq ch_t_parser (fp state'2 data'2) bytes2 in
-              match (parse ch_t_parser bytes2) with | Some (ch'2, l'2) -> let bytes'2 : bytes = Seq.slice bytes2 l'2 (Seq.length bytes2) in
-              let fp' = fp state'1 in
-              assert (cases_injective2_precond (parse_automata_gt state'1) fp' data'1 data'2 ch'1 ch'2 bytes'1 bytes'2);
-              assert (data'1 = data'2);
-              lemma_update_next_inj2 state data1 data2 ch1 ch2
-            )
-            else
-            (
-              let _ = cases_injective2_weaken (parse_automata_gt state'1) (fp state'1) in
-              let p1 = ch_t_parser `and_then` (fp state'1 data'1) in
-              let ret1' = 
-                parse_cast_inverse
-                ret_t
-                (post_t state'1 data'1)
-                (post_t state data1)
-                (lemma_cast_ret state data1 ch1)
-                p1
-                bytes1
-                ret1
-                l1
-              in
-              let _ = cases_injective2_weaken (parse_automata_gt state'2) (fp state'2) in
-              let p2 = ch_t_parser `and_then` (fp state'2 data'2) in
-              let ret2' = 
-                parse_cast_inverse
-                ret_t
-                (post_t state'2 data'2)
-                (post_t state data2)
-                (lemma_cast_ret state data2 ch2)
-                p2
-                bytes2
-                ret2
-                l2
-              in
-              lemma_update_next_non_intersect state data1 data2 ch1 ch2 ret1' ret2'
-            )
-          )
-        )
-        )
+    (
+      let s' = cp.next_state s ch1 in
+      let x' = dp.update_next s x ch1 in
+      let _ = bp.ch_t_bare_parser_valid b1 in
+      let (b'1 : bytes{Seq.length b'1 < Seq.length b1}) = Seq.slice b1 l01 (Seq.length b1) in
+      let _ = bp.ch_t_bare_parser_valid b2 in
+      let (b'2 : bytes{Seq.length b'2 < Seq.length b2}) = Seq.slice b2 l01 (Seq.length b2) in
+      automata_bare_parser'_pf2_aux cp dp bp pp s' x' b'1 b'2
     )
 
-let rec parse_automata'' 
-  (state : control_t)
-: Pure (parse_automata_type state)
-  (requires True)
-  (ensures (fun p -> parse_automata_spec state p))
-  (decreases %[ord state]) 
-= let _ = lemma_parse_automata'_inj2 state (parse_automata'') in
-  parse_automata' state (parse_automata'')
+let automata_bare_parser'_pf2
+  (cp : automata_control_param)
+  (dp : automata_data_param cp)
+  (bp : automata_bare_parser_param cp)
+  (pp : automata_parser_param cp dp bp)
+  (s : cp.control_t)
+  (x : dp.partial_t {dp.pre_t s x})
+: Lemma (no_lookahead (automata_bare_parser' cp dp bp s x))
+= Classical.forall_intro_2 (fun b1 b2 -> Classical.move_requires (automata_bare_parser'_pf2_aux cp dp bp pp s x b1) b2)
 
-assume val initial_state : control_t
+let rec automata_bare_parser'_pf3_aux
+  (cp : automata_control_param)
+  (dp : automata_data_param cp)
+  (bp : automata_bare_parser_param cp)
+  (pp : automata_parser_param cp dp bp)
+  (s : cp.control_t)
+  (x : dp.partial_t {dp.pre_t s x})
+  (b1 : bytes)
+  (b2 : bytes)
+: Lemma (requires injective_precond (automata_bare_parser' cp dp bp s x) b1 b2)
+        (ensures injective_postcond (automata_bare_parser' cp dp bp s x) b1 b2)
+        (decreases (Seq.length b1))
+= let p = automata_bare_parser' cp dp bp s x in
+  let _ = pp.ch_t_parser_valid () in
+  let _ = parser_kind_prop_equiv automata_default_parser_kind bp.ch_t_bare_parser in
+  match (parse p b1) with | Some (ret1, l1) ->
+  match (parse p b2) with | Some (ret2, l2) ->
+  match (parse (bp.ch_t_bare_parser) b1) with | Some (ch1, l01) ->
+  match (parse (bp.ch_t_bare_parser) b2) with | Some (ch2, l02) ->
+  let _ = 
+    Seq.lemma_split (Seq.slice b1 0 l1) l01;
+    Seq.lemma_split (Seq.slice b2 0 l2) l02
+  in
+  if cp.fail_check s ch1 then
+    _
+  else if cp.fail_check s ch2 then
+    _
+  else if cp.termination_check s ch1 then
+  (
+    if cp.termination_check s ch2 then
+    (
+      pp.lemma_update_term_inj2 s x x ch1 ch2;
+      assert (injective_precond bp.ch_t_bare_parser b1 b2);
+      assert ((l01 <: nat) = (l02 <: nat))
+    )
+    else
+      pp.lemma_update_term_next_non_intersect s x x ch1 ch2 ret1 ret2
+  )
+  else
+  (
+    if cp.termination_check s ch2 then
+      pp.lemma_update_term_next_non_intersect s x x ch2 ch1 ret2 ret1
+    else
+    (
+      let s'1 = cp.next_state s ch1 in
+      let s'2 = cp.next_state s ch2 in
+      let x'1 = dp.update_next s x ch1 in
+      let x'2 = dp.update_next s x ch2 in
+      let _ = bp.ch_t_bare_parser_valid b1 in
+      let (b'1 : bytes{Seq.length b'1 < Seq.length b1}) = Seq.slice b1 l01 (Seq.length b1) in
+      let _ = bp.ch_t_bare_parser_valid b2 in
+      let (b'2 : bytes{Seq.length b'2 < Seq.length b2}) = Seq.slice b2 l02 (Seq.length b2) in
+      if s'1 = s'2 then
+      (
+        let _ = automata_bare_parser'_pf1_aux cp dp bp pp s'1 x'1 x'2 b'1 b'2 in
+        pp.lemma_update_next_inj2 s x x ch1 ch2;
+        assert (injective_precond bp.ch_t_bare_parser b1 b2);
+        assert ((l01 <: nat) = (l02 <: nat));
+        let _ = automata_bare_parser'_pf3_aux cp dp bp pp s'1 x'1 b'1 b'2 in
+        _
+      )
+      else
+      (
+        pp.lemma_update_next_non_intersect s x x ch1 ch2 ret1 ret2
+      )
+    )
+  )
 
-assume val initial_data : (data : partial_t {pre_t initial_state data})
+let automata_bare_parser'_pf3
+  (cp : automata_control_param)
+  (dp : automata_data_param cp)
+  (bp : automata_bare_parser_param cp)
+  (pp : automata_parser_param cp dp bp)
+  (s : cp.control_t)
+  (x : dp.partial_t {dp.pre_t s x})
+: Lemma (injective (automata_bare_parser' cp dp bp s x))
+= Classical.forall_intro_2 (fun b1 b2 -> Classical.move_requires (automata_bare_parser'_pf3_aux cp dp bp pp s x b1) b2)
 
-let parse_automata = parse_automata'' initial_state initial_data
-*)
+let automata_bare_parser'_pf23
+  (cp : automata_control_param)
+  (dp : automata_data_param cp)
+  (bp : automata_bare_parser_param cp)
+  (pp : automata_parser_param cp dp bp)
+  (s : cp.control_t)
+  (x : dp.partial_t {dp.pre_t s x})
+: Lemma (parser_kind_prop automata_default_parser_kind (automata_bare_parser' cp dp bp s x))
+= parser_kind_prop_equiv automata_default_parser_kind (automata_bare_parser' cp dp bp s x);
+  automata_bare_parser'_pf2 cp dp bp pp s x;
+  automata_bare_parser'_pf3 cp dp bp pp s x
+ 
+let automata_bare_parser'_pf
+  (cp : automata_control_param)
+  (dp : automata_data_param cp)
+  (bp : automata_bare_parser_param cp)
+  (pp : automata_parser_param cp dp bp)
+: Lemma (
+  (forall s. and_then_cases_injective_dep (dp.post_t s) (automata_bare_parser' cp dp bp s)) /\
+  (forall s data. parser_kind_prop automata_default_parser_kind (automata_bare_parser' cp dp bp s data)))
+= Classical.forall_intro (fun s -> automata_bare_parser'_pf1 cp dp bp pp s);
+  Classical.forall_intro_2 (fun s data -> automata_bare_parser'_pf23 cp dp bp pp s data)
+  
+let automata_parser
+  (cp : automata_control_param)
+  (dp : automata_data_param cp)
+  (bp : automata_bare_parser_param cp)
+  (pp : automata_parser_param cp dp bp)
+  (s : cp.control_t)
+  (data : dp.partial_t {dp.pre_t s data})
+: (parser automata_default_parser_kind (ret : dp.ret_t {dp.post_t s data ret}))
+= let _ = automata_bare_parser'_pf cp dp bp pp in
+  automata_bare_parser' cp dp bp s data
+  
